starting the proof of subject reduction

theories/MetaTheory/Typing.v
@@ -19,13 +19,9 @@ Proof.
 induction t using term_ind' in s', ρ |- * ; simpl_subst ; cbn ; auto.
 Qed.*)
 
-(** [All_context P Γ] means that [P Γ' ty] holds on every type [Γ' ⊢ ty]
-    in the context [Γ]. *)
-Inductive All_context {s} (P : forall s', context s s' -> term s' -> Prop) :
-  forall {s'}, context s s' -> Prop :=
-| All_context_nil : All_context P CNil
-| All_context_cons {s'} Γ x (ty : term s') :
-    All_context P Γ -> P s' Γ ty -> All_context P (CCons Γ x ty).
+(***********************************************************************)
+(** * Lifting a property on a spine of arguments. *)
+(***********************************************************************)
 
 Section All_spine.
   Context (P : forall s, evar_map -> context ∅ s -> term s -> term s -> Prop).
@@ -34,15 +30,58 @@ Section All_spine.
       then [All_spine Σ Γ f_ty args T] means that appling a function of type [f_ty]
       to the list of arguments [args] yields a term of type [T]. *)
   Inductive All_spine {s} (Σ : evar_map) (Γ : context ∅ s) : term s -> list (term s) -> term s -> Prop :=
-  | All_spine_nil f_ty :
-      All_spine Σ Γ f_ty [] f_ty
+  | All_spine_nil f_ty f_ty' :
+      Σ ⊢ f_ty ≡ f_ty' ->
+      All_spine Σ Γ f_ty [] f_ty'
 
   | All_spine_cons f_ty x a b arg args T :
       P s Σ Γ (TProd x a b) TType ->
       Σ ⊢ f_ty ≡ TProd x a b ->
+      P s Σ Γ arg a ->
       All_spine Σ Γ (b[x := arg]) args T ->
       All_spine Σ Γ f_ty (arg :: args) T.
 End All_spine.
+
+Derive Signature for All_spine.
+
+Lemma All_spine_consequence (P Q : forall s, evar_map -> context ∅ s -> term s -> term s -> Prop) :
+  (forall s Σ Γ t T, P s Σ Γ t T -> Q s Σ Γ t T) ->
+  forall s Σ Γ f_ty args (T : term s),
+    All_spine P Σ Γ f_ty args T ->
+    All_spine Q Σ Γ f_ty args T.
+Proof.
+intros Himpl s Σ Γ f_ty args T H. induction H ; econstructor ; eauto.
+Qed.
+
+Lemma All_spine_conv_type P {s} Σ Γ f_ty args (T T' : term s) :
+  All_spine P Σ Γ f_ty args T ->
+  Σ ⊢ T ≡ T' ->
+  All_spine P Σ Γ f_ty args T'.
+Proof.
+intros H. induction H.
+- intros H1. constructor. now rewrite <-H1.
+- intros H3. econstructor ; eauto.
+Qed.
+
+Lemma All_spine_conv_func_type P {s} Σ Γ f_ty f_ty' args (T : term s) :
+  All_spine P Σ Γ f_ty args T ->
+  Σ ⊢ f_ty ≡ f_ty' ->
+  All_spine P Σ Γ f_ty' args T.
+Proof.
+intros H. induction H.
+- intros H1. constructor. now rewrite <-H1.
+- intros H3. econstructor ; eauto. now rewrite <-H3.
+Qed.
+
+#[export] Instance All_spine_proper_conv_type P s Σ Γ :
+  Proper (conv Σ ==> eq ==> conv Σ ==> iff) (@All_spine s P Σ Γ).
+Proof.
+intros f_ty f_ty' Hfty args args' <- T T' HT. split ; intros H.
+- revert HT. apply All_spine_conv_type.
+  revert Hfty. now apply All_spine_conv_func_type.
+- symmetry in HT, Hfty. revert HT. apply All_spine_conv_type.
+  revert Hfty. now apply All_spine_conv_func_type.
+Qed.
 
 (***********************************************************************)
 (** * Typing relation. *)
@@ -50,9 +89,6 @@ End All_spine.
 
 Reserved Notation "Σ ;; Γ ⊢ t : T"
   (at level 50, no associativity, Γ at next level, t at next level, T at next level).
-
-Reserved Notation "'typing_context' Σ Γ"
-  (at level 9, no associativity, Σ at next level, Γ at next level).
 
 Unset Elimination Schemes.
 
@@ -81,7 +117,7 @@ Inductive typing {s} (Σ : evar_map) (Γ : context ∅ s) : term s -> term s -> 
 | typing_app f f_ty args T :
     Σ ;; Γ ⊢ f : f_ty ->
     (*is_TApp f = false ->*)
-    args <> [] ->
+    (*args <> [] ->*)
     All_spine (@typing) Σ Γ f_ty args T ->
     Σ ;; Γ ⊢ TApp f args : T
 
@@ -103,6 +139,10 @@ Set Elimination Schemes.
 
 Derive Signature for typing.
 
+(***********************************************************************)
+(** * Typing renamings and substitutions. *)
+(***********************************************************************)
+
 (** [Σ ;; Γ ⊢ᵣ ρ : Δ] means that the renaming [ρ] maps well-typed terms
     in context [Γ] to well-typed terms in context [Δ]. *)
 Definition typing_ren {s s'} (Σ : evar_map) (Γ : context ∅ s) (ρ : ren s s') (Δ : context ∅ s') :=
@@ -118,6 +158,46 @@ Definition typing_subst {s s'} Σ (Γ : context ∅ s) (σ : subst s s') (Δ : c
 
 Notation "Σ ;; Γ ⊢ₛ σ : Δ" := (typing_subst Σ Γ σ Δ)
   (at level 50, Γ at next level, σ at next level, Δ at next level).
+
+(***********************************************************************)
+(** * Typing local contexts. *)
+(***********************************************************************)
+
+(** [typing_context Σ Γ] means that the types in context [Γ] are well-typed. *)
+Inductive typing_context (Σ : evar_map) : forall {s}, context ∅ s -> Prop :=
+| typing_context_nil : typing_context Σ CNil
+| typing_context_cons {s} Γ x (ty : term s) :
+    typing_context Σ Γ ->
+    Σ ;; Γ ⊢ ty : TType ->
+    typing_context Σ (CCons Γ x ty).
+
+(***********************************************************************)
+(** * Typing evar-maps. *)
+(***********************************************************************)
+
+(** [typing_evar_entry Σ e] asserts that the evar-entry [e] is well-typed
+    in evar-map [Σ]. *)
+Inductive typing_evar_entry (Σ : evar_map) : evar_entry -> Prop :=
+
+(** An undefined evar entry is well-typed if the type if well-typed. *)
+| typing_evar_undefined ty :
+    Σ ;; CNil ⊢ ty : TType ->
+    typing_evar_entry Σ (mk_evar_entry ty None)
+
+(** A defined evar entry is well-typed if the type is well-typed
+    and the definition has the correct type. *)
+| typing_evar_defined ty def :
+    Σ ;; CNil ⊢ ty : TType ->
+    Σ ;; CNil ⊢ def : ty ->
+    typing_evar_entry Σ (mk_evar_entry ty (Some def)).
+
+Derive Signature for typing_evar_entry.
+
+(** [typing_evar_map Σ] means that the evar-map [Σ] is well-typed.
+    We do _not_ check that the evar-map is acyclic:
+    this would likely be very annoying to do. *)
+Definition typing_evar_map (Σ : evar_map) :=
+  forall ev entry, Σ ev = Some entry -> typing_evar_entry Σ entry.
 
 (***********************************************************************)
 (** * Induction principle for [typing]. *)
@@ -139,7 +219,7 @@ Lemma typing_ind
   (Happ : forall s Σ Γ f f_ty args T,
     Σ ;; Γ ⊢ f : f_ty -> P s Σ Γ f f_ty ->
     (*is_TApp f = false ->*)
-    args <> [] ->
+    (*args <> [] ->*)
     All_spine (fun s Σ Γ t T => Σ ;; Γ ⊢ t : T /\ P s Σ Γ t T) Σ Γ f_ty args T ->
     P s Σ Γ (TApp f args) T)
   (Hevar : forall s Σ Γ ev entry,
@@ -157,10 +237,11 @@ fix IH 6. intros s Σ Γ t T H. depelim H.
 - now apply Hvar.
 - apply Hlam ; auto.
 - apply Hprod ; auto.
-- apply Happ with f_ty ; auto. clear f H H0. revert f_ty args T H1.
-  fix IHspine 4. intros f_ty args T H1. destruct H1.
-  + constructor.
-  + econstructor ; [|eassumption|].
+- apply Happ with f_ty ; auto. clear f H. revert f_ty args T H0.
+  fix IHspine 4. intros f_ty args T H0. destruct H0.
+  + constructor. assumption.
+  + econstructor ; [| eassumption | |].
+    * split ; [assumption |]. now apply IH.
     * split ; [assumption |]. apply IH. assumption.
     * apply IHspine ; auto.
 - apply Hevar ; auto.
@@ -168,7 +249,107 @@ fix IH 6. intros s Σ Γ t T H. depelim H.
 Qed.
 
 (***********************************************************************)
-(** * Compatibility of typing with renaming and substitution. *)
+(** * Inverting typing derivations. *)
+(***********************************************************************)
+
+(** Inverting typing derivations is not completely trivial:
+    indeed typing looks syntax directed at first glance, but in fact
+    it is _not_ because of the rule [typing_conv_type]. *)
+
+Lemma typing_type_inv {s} Σ Γ T :
+  Σ ;; Γ ⊢ TType : T ->
+  Σ ⊢ T ≡ @TType s.
+Proof.
+intros H. depind H.
+- reflexivity.
+- now rewrite <-H0.
+Qed.
+
+Lemma typing_var_inv {s} Σ Γ (i : index s) T :
+  Σ ;; Γ ⊢ TVar i : T ->
+  Σ ⊢ T ≡ lookup_context i Γ.
+Proof.
+intros H. depind H.
+- now rewrite H.
+- now rewrite <-H0.
+Qed.
+
+Lemma typing_lam_inv_aux {s x} Σ Γ (t : term s) T :
+  Σ ;; Γ ⊢ t : T ->
+  forall ty body, t = TLam x ty body ->
+  exists body_ty,
+    Σ ⊢ T ≡ TProd x ty body_ty /\
+    Σ ;; Γ ⊢ ty : TType /\
+    Σ ;; CCons Γ x ty ⊢ body : body_ty.
+Proof.
+intros H. induction H ; intros ty' body' Ht ; depelim Ht.
+- exists body_ty. now split3.
+- destruct (IHtyping1 ty' body' eq_refl) as (body_ty' & HA & Hty & Hbody).
+  exists body_ty'. split3 ; auto. now rewrite <-H0.
+Qed.
+
+Lemma typing_lam_inv {s x} Σ Γ (ty : term s) body T :
+  Σ ;; Γ ⊢ TLam x ty body : T ->
+  exists body_ty,
+    Σ ⊢ T ≡ TProd x ty body_ty /\
+    Σ ;; Γ ⊢ ty : TType /\
+    Σ ;; CCons Γ x ty ⊢ body : body_ty.
+Proof. intros H. eapply typing_lam_inv_aux ; eauto. Qed.
+
+Lemma typing_prod_inv_aux {s x} Σ Γ (t : term s) T :
+  Σ ;; Γ ⊢ t : T ->
+  forall a b, t = TProd x a b ->
+    Σ ⊢ T ≡ TType /\
+    Σ ;; Γ ⊢ a : TType /\
+    Σ ;; CCons Γ x a ⊢ b : TType.
+Proof.
+intros H. induction H ; intros a' b' Ht ; depelim Ht.
+- now split3.
+- destruct (IHtyping1 a' b' eq_refl) as (HA & Ha & Hb).
+  split3 ; auto. now rewrite <-H0.
+Qed.
+
+Lemma typing_prod_inv {s x} Σ Γ (a : term s) b T :
+  Σ ;; Γ ⊢ TProd x a b : T ->
+  Σ ⊢ T ≡ TType /\ Σ ;; Γ ⊢ a : TType /\ Σ ;; CCons Γ x a ⊢ b : TType.
+Proof. intros H. eapply typing_prod_inv_aux ; eauto. Qed.
+
+Lemma typing_app_inv_aux {s} Σ Γ t (T : term s) :
+  Σ ;; Γ ⊢ t : T ->
+  forall f args, t = TApp f args ->
+  exists f_ty,
+    Σ ;; Γ ⊢ f : f_ty /\
+    All_spine (@typing) Σ Γ f_ty args T.
+Proof.
+intros H. induction H ; intros f' args' Ht ; depelim Ht.
+- exists f_ty. split ; auto. revert H0.
+  apply All_spine_consequence. clear. firstorder.
+- destruct (IHtyping1 f' args' eq_refl) as (f_ty' & Hf & H3).
+  exists f_ty'. split ; auto. clear IHtyping1 IHtyping2 H H1 Hf.
+  depind H3 ; econstructor ; eauto. now rewrite H.
+Qed.
+
+Lemma typing_app_inv {s} Σ Γ f args (T : term s) :
+  Σ ;; Γ ⊢ TApp f args : T ->
+  exists f_ty,
+    Σ ;; Γ ⊢ f : f_ty /\
+    All_spine (@typing) Σ Γ f_ty args T.
+Proof. intros H. eapply typing_app_inv_aux ; eauto. Qed.
+
+Lemma typing_evar_inv {s} Σ Γ ev (T : term s) :
+  Σ ;; Γ ⊢ TEvar ev : T ->
+  exists entry,
+    Σ ev = Some entry /\
+    Σ ⊢ T ≡ wk entry.(evar_type).
+Proof.
+intros H. depind H.
+- exists entry. now split.
+- destruct IHtyping1 as (entry & H2 & H3). exists entry.
+  split ; auto. now rewrite <-H0.
+Qed.
+
+(***********************************************************************)
+(** * Compatibility of typing with renaming. *)
 (***********************************************************************)
 
 Lemma typing_rid {s} Σ (Γ : context ∅ s) :
@@ -221,17 +402,19 @@ intros Ht Hρ. induction Ht in s', ρ, Δ, Hρ |- * ; simpl_subst.
 - apply typing_prod ; auto using typing_rup.
 - eapply typing_app.
   + now apply IHHt.
-  + now depelim args.
-  + clear H IHHt Ht. depind H0 ; cbn.
-    * constructor.
-    * destruct H as [H H'].
-      apply All_spine_cons with (x := x) (a := rename ρ a) (b := rename (rup x ρ) b).
-      --simpl_subst in H'. now apply H'.
-      --rewrite H0. now simpl_subst.
-      --simpl_subst. simpl_subst in IHAll_spine. now apply IHAll_spine.
+  + clear IHHt Ht. depind H ; cbn ; [constructor ; now rewrite H |].
+    apply All_spine_cons with (x := x) (a := rename ρ a) (b := rename (rup x ρ) b).
+    * simpl_subst in H. now apply H.
+    * rewrite H0. now simpl_subst.
+    * now apply H1.
+    * simpl_subst. simpl_subst in IHAll_spine. apply IHAll_spine ; auto.
 - now apply typing_evar.
 - apply typing_conv_type with (A := rename ρ A) ; auto. now rewrite H.
 Qed.
+
+(***********************************************************************)
+(** * Compatibility of typing with substitution. *)
+(***********************************************************************)
 
 Lemma typing_sid {s} Σ (Γ : context ∅ s) :
   Σ ;; Γ ⊢ₛ sid : Γ.
@@ -283,12 +466,12 @@ intros Ht Hσ. induction Ht in s', σ, Δ, Hσ |- * ; simpl_subst.
 - apply typing_lam ; auto using typing_sup.
 - apply typing_prod ; auto using typing_sup.
 - apply typing_app with (f_ty := substitute σ f_ty) ; auto.
-  + depelim args ; auto. intros H' ; depelim H'.
-  + clear f Ht IHHt H. depind H0 ; [constructor |]. cbn.
-    apply All_spine_cons with (x := x) (a := substitute σ a) (b := substitute (sup x σ) b).
-    * simpl_subst in H. now apply H.
-    * rewrite H0. simpl_subst. reflexivity.
-    * simpl_subst. simpl_subst in IHAll_spine. now apply IHAll_spine.
+  clear f Ht IHHt. depind H ; [constructor ; now rewrite H |]. cbn.
+  apply All_spine_cons with (x := x) (a := substitute σ a) (b := substitute (sup x σ) b).
+  + simpl_subst in H. now apply H.
+  + rewrite H0. simpl_subst. reflexivity.
+  + now apply H1.
+  + simpl_subst. simpl_subst in IHAll_spine. now apply IHAll_spine.
 - econstructor ; eauto.
 - eapply typing_conv_type ; eauto. now rewrite H.
 Qed.
@@ -312,20 +495,125 @@ intros H1 H2 i. simpl_subst. rewrite <-substitute_substitute.
 eapply typing_substitute ; eauto.
 Qed.
 
-(** Next define typing on evar-maps... *)
+(***********************************************************************)
+(** * Properties of typing. *)
+(***********************************************************************)
 
+Lemma typing_lookup_context {s} Σ (Γ : context ∅ s) i :
+  typing_context Σ Γ ->
+  Σ ;; Γ ⊢ lookup_context i Γ : TType.
+Proof.
+intros H. induction H.
+- depelim i.
+- depelim i ; simp lookup_context ; simpl_subst.
+  + change TType with (rename (@rshift s x) TType).
+    eapply typing_rename ; eauto. apply typing_rshift.
+  + change TType with (rename (@rshift s x) TType).
+    eapply typing_rename ; eauto. apply typing_rshift.
+Qed.
 
-Lemma typing_type_ok {s} Σ Γ (t T : term s) :
-  Σ ;; Γ ⊢ t : T ->
+Lemma typing_evar_type Σ entry :
+  typing_evar_entry Σ entry ->
+  Σ ;; CNil ⊢ entry.(evar_type) : TType.
+Proof. intros H. destruct H ; cbn ; assumption. Qed.
+
+(** Beta reduction preserves typing. *)
+Lemma typing_beta {s} Σ Γ x ty body arg args (T : term s) :
+  Σ ;; Γ ⊢ TApp (TLam x ty body) (arg :: args) : T ->
+  Σ ;; Γ ⊢ TApp (body[x := arg]) args : T.
+Proof.
+intros H. apply typing_app_inv in H. destruct H as (f_ty & H1 & H2).
+apply typing_lam_inv in H1. destruct H1 as (body_ty & H1 & Hty & Hbody).
+depelim H2. assert (x0 = x) as ->. { destruct x0 ; destruct x ; reflexivity. }
+rewrite H1 in H0. clear f_ty H1. apply conv_prod_inv in H0. destruct H0 as (H4 & H5).
+eapply typing_app with (body_ty[x := arg]).
+- eapply typing_substitute ; eauto. apply typing_scons ; simpl_subst.
+  + apply typing_conv_type with a ; auto. now symmetry.
+  + apply typing_sid.
+- rewrite H5. assumption.
+Qed.
+
+Lemma typing_evar_expand_helper {s} Σ Γ ev (T : term s) :
+  typing_evar_map Σ ->
+  Σ ;; Γ ⊢ TEvar ev : T ->
   Σ ;; Γ ⊢ T : TType.
-Proof. Admitted.
+Proof.
+intros HΣ H. depind H.
+- change TType with (@wk ∅ s _ TType). unfold wk. eapply typing_rename.
+  + apply typing_evar_type. apply (HΣ ev entry H).
+  + intros i. depelim i.
+- assumption.
+Qed.
+
+(** Evar expansion preserves typing. *)
+Lemma typing_evar_expand {s} Σ Γ ev ty def (T : term s) :
+  typing_evar_map Σ ->
+  Σ ;; Γ ⊢ TEvar ev : T ->
+  Σ ev = Some (mk_evar_entry ty (Some def)) ->
+  Σ ;; Γ ⊢ wk def : T.
+Proof.
+intros H1 H2 H3. pose proof (HT := typing_evar_expand_helper _ _ _ _ H1 H2).
+specialize (H1 _ _ H3). depelim H1.
+apply typing_evar_inv in H2. destruct H2 as (entry & H4 & H5).
+rewrite H4 in H3. depelim H3. cbn in H5. apply typing_conv_type with (wk ty).
+- unfold wk. eapply typing_rename ; eauto. intros i. depelim i.
+- now symmetry.
+- assumption.
+Qed.
 
 (** Reducing a term doesn't change its type. *)
-Lemma typing_red {s} Σ Γ (t u T : term s) :
+Lemma typing_red1 {s} Σ Γ (t u T : term s) :
+  typing_evar_map Σ ->
+  typing_context Σ Γ ->
   Σ ;; Γ ⊢ t : T ->
-  Σ ⊢ t ~> u ->
+  Σ ⊢ t ~>₁ u ->
   Σ ;; Γ ⊢ u : T.
-Proof. Admitted.
+Proof.
+intros HΣ HΓ Ht Hred. depind Hred.
+- eapply typing_beta ; eauto.
+- eapply typing_evar_expand ; eauto.
+- (*apply typing_lam_inv in Ht. destruct Ht as (body_ty & H1 & Hty & Hbody).
+  apply IHHred in Hty ; auto. rewrite Hred in H1.
+  apply typing_conv_type with (TProd x ty' body_ty).
+  + apply typing_lam.
+    * assumption.
+    *
+
+  apply typing_lam. apply IHHred.*)
+
+
+apply HΣ in H. depelim H.  depelim Ht. apply typing_evar_entry.
+
+Admitted.
+
+(** In a typing derivation, the type is itself well-typed. *)
+Lemma typing_type_ok {s} Σ Γ (t T : term s) :
+  typing_evar_map Σ ->
+  typing_context Σ Γ ->
+  Σ ;; Γ ⊢ t : T ->
+  Σ ;; Γ ⊢ T : TType.
+Proof.
+intros Hevm Hctx Ht. induction Ht.
+- constructor.
+- rewrite <-H. now apply typing_lookup_context.
+- constructor ; auto. apply IHHt2 ; auto. constructor ; auto.
+- constructor.
+- clear f H Ht. depind H0 ; [auto |]. apply IHAll_spine. intros _ _.
+  destruct H as [H _].
+  assert (Σ ;; Γ ⊢ a : TType) by admit.
+  assert (Σ ;; CCons Γ x a ⊢ b : TType) by admit.
+  change TType with (TType [x := arg]). eapply typing_substitute.
+  + eassumption.
+  + apply typing_scons.
+    * simpl_subst. apply H1.
+    * apply typing_sid.
+- unfold wk. change (@TType s) with (@rename ∅ s wk_idx TType).
+  eapply typing_rename.
+  + apply typing_evar_type. now apply (Hevm ev).
+  + intros i. depelim i.
+- assumption.
+Admitted.
+
 
 (** Changing a term to a convertible one doesn't change its type. *)
 Lemma typing_conv {s} Σ Γ (t u T : term s) :
@@ -333,3 +621,9 @@ Lemma typing_conv {s} Σ Γ (t u T : term s) :
   Σ ⊢ t ≡ u ->
   Σ ;; Γ ⊢ u : T.
 Proof. Admitted.
+
+#[export] Instance typing_conv_Proper {s} Σ Γ :
+  Proper (conv Σ ==> eq ==> iff) (@typing s Σ Γ).
+Proof.
+intros t t' Ht T T' ->. split ; intros H ; eapply typing_conv ; eauto. now symmetry.
+Qed.
